

Lecture 7

Sigma Notation Σ

The summation symbol
(Greek letter sigma) — \sum — a_k is a formula for the k th term.

n — The index k ends at $k = n$.

$k = 1$ — The index k starts at $k = 1$.

$$\sum_{k=1}^{k=6} k^2 = 1^2 + 2^2 + 3^2 + 4^2 + 5^2 + 6^2$$

$$\sum_{k=1}^n k = \frac{n(n+1)}{2} = \frac{n^2 + n}{2}$$

$$\sum_{k=1}^n k^2 = \frac{n(n+1)(2n+1)}{6}$$

$$\sum_{k=1}^n k^3 = \frac{n^2(n+1)^2}{4}$$

$$\sum_{k=1}^n \frac{1}{n} = n \frac{1}{n} = 1$$

Example

If $f(x) = 1 - x^2$

Find $\lim_{n \rightarrow \infty} \left[\sum_{k=1}^n f\left(\frac{k}{n}\right) \left(\frac{1}{n}\right) \right]$

Solution

$$\begin{aligned} f\left(\frac{k}{n}\right) &= 1 - \left(\frac{k}{n}\right)^2 \\ \sum_{k=1}^n f\left(\frac{k}{n}\right) \left(\frac{1}{n}\right) &= \sum_{k=1}^n \left\{ \left(1 - \left(\frac{k}{n}\right)^2\right) \left(\frac{1}{n}\right) \right\} \\ &= \sum_{k=1}^n \left\{ \frac{1}{n} - \frac{k^2}{n^3} \right\} \\ &= \sum_{k=1}^n \frac{1}{n} - \sum_{k=1}^n \frac{k^2}{n^3} \end{aligned}$$

$$= \sum_{k=1}^n \frac{1}{n} - \frac{1}{n^3} \sum_{k=1}^n k^2$$

$$\sum_{k=1}^n \frac{1}{n} = \boldsymbol{n} \frac{1}{n} = 1,$$

$$\sum_{k=1}^n k^2 = \frac{\boldsymbol{n}(\boldsymbol{n} + 1)(2\boldsymbol{n} + 1)}{6}$$

$$\sum_{k=1}^n f\left(\frac{k}{n}\right) \left(\frac{1}{n}\right) = 1 - \frac{n(n+1)(2n+1)}{6n^3}$$

$$= 1 - \frac{2n^3 + 3n^2 + n}{6n^3}$$

$$\lim_{n \rightarrow \infty} \left[\sum_{k=1}^n f\left(\frac{k}{n}\right) \left(\frac{1}{n}\right) \right]$$

$$= \lim_{n \rightarrow \infty} \left[1 - \frac{2n^3 + 3n^2 + n}{6n^3} \right]$$

$$= 1 - \frac{2}{6} = \frac{2}{3}$$

Example

Prove that

$$\sum_{n=1}^m \frac{1}{n(n+1)} = \frac{m}{m+1}$$

From partial fractions

$$\frac{1}{n(n+1)} = \frac{1}{n} - \frac{1}{n+1}$$

Solution

$$\begin{aligned}\sum_1^m \frac{1}{n(n+1)} &= \sum_1^m \frac{1}{n} - \sum_1^m \frac{1}{n+1} \\&= \left(1 + \frac{1}{2} + \frac{1}{3} + \cdots + \frac{1}{m}\right) - \left(\frac{1}{2} + \frac{1}{3} + \cdots + \frac{1}{m+1}\right) \\&= 1 - \frac{1}{m+1} = \frac{m}{m+1}\end{aligned}$$

Changing Index in the sigma notation

Example

Change the lower index of the sum

$$\sum_{k=1}^{k=n} a_{k-1} \quad a_{n-k}$$

to start with $j = 3$

old $k = 1, 2, 3 \dots$

new $j = 3, 4, 5 \dots$

$$j = k + 2 \rightarrow k = j - 2$$

$$\sum_{k=1}^{k=n} a_{k-1} a_{n-k} = \sum_{j-2=1}^{j-2=n} a_{j-2-1} a_{n-j+2} = \sum_{j=3}^{j=n+2} a_{j-3} a_{n-j+2}$$

Example

Change the lower index of the sum

$$\sum_{k=5}^{k=n} a_{n+k} \quad b_{n-k}$$

to start with $j = 0$

old $k = 5, 6, 7 \dots$

new $j = 0, 1, 2 \dots$

$$k = j + 5$$

$$\sum_{k=5}^{k=n} a_{n+k} b_{n-k} = \sum_{j+5=5}^{j+5=n} a_{n+j+5} b_{n-j-5} = \sum_{j=0}^{j=n-5} a_{n+j+5} b_{n-j-5}$$

Series

A series is the sum of a sequence.

□ The infinite sequence

$$\{a_n\}_1^\infty = \{a_1, a_2, a_3, \dots\}$$

□ The infinite series

$$a_1 + a_2 + a_3 + \dots$$

Partial sums

□ Infinite series $a_1 + a_2 + a_3 + \cdots$

$$S_1 = a_1$$

$$S_2 = a_1 + a_2$$

$$S_3 = a_1 + a_2 + a_3$$

$$S_4 = a_1 + a_2 + a_3 + a_4$$

$$\vdots$$

$$S_n = a_1 + a_2 + a_3 + a_4 + \cdots + a_n$$

□ The sequence of partial sum

$$S_n = \{S_1, S_2, S_3, S_4, \dots, S_n, \dots\}$$

The sum S of the infinite series

$$S = \sum_{n=1}^{\infty} a_n = \lim_{n \rightarrow \infty} S_n$$

□ The infinite sequence $\left(\frac{3}{10}, \frac{3}{10^2}, \frac{3}{10^3}, \dots, \frac{3}{10^n}, \dots\right)$
 □ The infinite series $\frac{3}{10} + \frac{3}{10^2} + \frac{3}{10^3} + \dots + \frac{3}{10^n} + \dots$

$$S_1 = a_1 = 0.3$$

$$S_2 = a_1 + a_2 = 0.3 + 0.03 = 0.33$$

$$S_3 = a_1 + a_2 + a_3 = 0.3 + 0.03 + 0.003 = 0.333$$

$$S_4 = a_1 + a_2 + a_3 + a_4 = 0.3 + 0.03 + 0.003 + 0.0003 = 0.3333$$

⋮

□ The sequence of partial sum

$$\begin{aligned} S_n &= \{S_1, S_2, S_3, S_4, \dots, S_n, \dots\} \\ &= \{0.3, 0.33, 0.333, 0.3333, \dots\} \end{aligned}$$

□ The sum S of the infinite series

$$S = 0.33333333 = \frac{1}{3}$$

Converges and diverges

Theorem

□ A series $\sum a_n$ is **convergent** (or **converges**) if its sequence of partial sums $\{S_n\}$ converges

$$\lim_{n \rightarrow \infty} S_n = S$$

□ The limit S is the **sum** of the series

$$S = a_1 + a_2 + a_3 + \cdots + a_n + \cdots$$

□ The series $\sum a_n$ is divergent (or diverges) if $\{S_n\}$ diverges. A divergent series has no sum.

Example

Given the series

$$\frac{1}{1 \times 2} + \frac{1}{2 \times 3} + \frac{1}{3 \times 4} + \dots + \frac{1}{n \times (n+1)} + \dots,$$

- a) Find $S_1, S_2, S_3, \dots, S_6,$ b) Find S_n
- c) Show that the series converges and find its sum.

Solution

a)

$$S_1 = a_1 = \frac{1}{1 \times 2} = \frac{1}{2}$$

$$S_2 = a_1 + a_2 = \frac{1}{1 \times 2} + \frac{1}{2 \times 3} = \frac{2}{3}$$

$$S_3 = a_1 + a_2 + a_3 = \frac{1}{1 \times 2} + \frac{1}{2 \times 3} + \frac{1}{3 \times 4} = \frac{3}{4}$$

$$S_4 = a_1 + a_2 + a_3 + a_4 = \frac{4}{5}$$

$$S_5 = a_1 + a_2 + a_3 + a_4 + a_5 = \frac{5}{6}$$

$$S_6 = a_1 + a_2 + a_3 + a_4 + a_5 + a_6 = \frac{6}{7}$$

b)

□ The **sequence** of partial sum

$$S_n = \{S_1, S_2, S_3, S_4, \dots, S_n, \dots\} = \left\{ \frac{1}{2}, \frac{2}{3}, \frac{3}{4}, \frac{4}{5}, \frac{5}{6}, \frac{6}{7}, \dots \right\}$$

□ The general formula for S_n

$$S_n = \frac{n}{n+1}$$

c)

Converges and its sum

$$\lim_{n \rightarrow \infty} S_n = \lim_{n \rightarrow \infty} \frac{n}{n+1} = 1$$

The **sum** of the series $S=1$

Geometric Series

$$a + ar + ar^2 + ar^3 + \dots + ar^{n-1} + \dots$$

□ converges if $|r| < 1$

$$S = \frac{a}{1 - r}$$

□ diverges if $|r| > 1$

Example

Prove that the following series converges and find its sum:

$$0.6 + 0.06 + 0.006 + \dots + \frac{6}{10^n} + \dots$$

The series is a geometric series $r = \frac{0.06}{0.6} = 0.1$

Since $|r| < 1 \rightarrow$ geometric series **convergent**

$$S = \frac{a}{1 - r} = \frac{0.6}{1 - 0.1} = \frac{2}{3}$$

$$0.6 + 0.06 + 0.006 + \dots + \frac{6}{10^n} + \dots = \frac{2}{3}$$

The ratio test for convergent

□ Convergent

$$\left| \frac{A_{n+1}}{A_n} \right| < 1.$$

□ Divergent

$$\left| \frac{A_{n+1}}{A_n} \right| > 1$$

□ Failed

$$\left| \frac{A_{n+1}}{A_n} \right| = 1.$$

Example

Find all values of x for which the following series will be convergent, and find its sum

$$\frac{1}{2} + \frac{(x-3)}{4} + \frac{(x-3)^2}{8} + \dots + \frac{(x-3)^n}{2^{n+1}} + \dots$$

Solution

The series to be convergent, it must satisfy the ratio test

$$\left| \frac{a_{n+1}}{a_n} \right| < 1$$

$$\left| \frac{(x-3)}{4} \div \frac{1}{2} \right| = \left| \frac{(x-3)}{2} \right| < 1$$

$$|x-3| < 2 \rightarrow -2 < x-3 < 2 \rightarrow 1 < x < 5$$

The series is a geometric series

$$a = 0.5 \qquad r = \frac{x-3}{2}$$

Thus, the sum is

$$S = \frac{a}{1-r} = \frac{0.5}{1-\frac{x-3}{2}} = \frac{1}{5-x}$$

Taylor Series

Any defined continuous function $f(x)$ can be approximated by **Taylor series** as:

$$\begin{aligned} f(x) = & f(x_0) + \frac{(x - x_0)}{1!} f'(x_0) \\ & + \frac{(x - x_0)^2}{2!} f''(x_0) \\ & + \frac{(x - x_0)^3}{3!} f'''(x_0) + \dots \end{aligned}$$

Maclaurin series is a **special case** of Taylor series

If $x_0 = 0$, then the **Taylor series** converts to the **Maclaurin series**

$$\begin{aligned} f(x) = & f(0) + \frac{x}{1!} f'(0) \\ & + \frac{x^2}{2!} f''(0) + \frac{x^3}{3!} f'''(0) + \dots \end{aligned}$$

Example

□ Use **Taylor** series to expand the function

$$f(x) = e^x \text{ with } x_0 = 0$$

□ Then prove that $0 \leq (1 + x)^m \leq e^{mx}$ for positive m and $x \geq -1$.

Solution

$$f(x) = e^x \text{ with } x_0 = 0$$

$$f(x) = e^x \quad \rightarrow \quad f(0) = e^0 = 1$$

$$f'(x) = e^x \quad \rightarrow \quad f'(0) = e^0 = 1$$

$$f''(x) = e^x \quad \rightarrow \quad f''(0) = e^0 = 1$$

$$f(x) = f(0) + \frac{x}{1!}f'(0) + \frac{x^2}{2!}f''(0) + \frac{x^3}{3!}f'''(0) + \dots$$

$$e^x = 1 + x + \frac{x^2}{2!} + \frac{x^3}{3!} + \dots$$

$$e^x = 1 + x + \frac{x^2}{2!} + \frac{x^3}{3!} + \dots$$

$$1 + x \leq e^x$$

$$0 \leq 1 + x \leq e^x$$

$$0 \leq (1 + x)^m \leq e^{mx}$$

Example

□ Use **Taylor** series to expand the function

$$f(x) = \sqrt[3]{x+1} \text{ with } x_0 = 0$$

$$f(x) = \sqrt[3]{x+1} \quad \rightarrow f(0) = 1$$

$$f'(x) = \frac{1}{3}(1+x)^{-\frac{2}{3}} \quad \rightarrow f'(0) = \frac{1}{3}$$

$$f''(x) = -\frac{2}{9}(1+x)^{-\frac{5}{3}} \quad \rightarrow f''(0) = -\frac{2}{9}$$

$$f'''(x) = \frac{10}{27}(1+x)^{-\frac{8}{3}} \quad \rightarrow f'''(0) = \frac{10}{27}$$

$$f(x) = f(0) + \frac{x}{1!}f'(0) + \frac{x^2}{2!}f''(0) + \frac{x^3}{3!}f'''(0) + \dots$$

$$f(x) = \sqrt[3]{x+1} = 1 + \frac{1}{3}x + \frac{-1}{9}x^2 + \frac{5}{81}x^3 + \dots$$

Exercises

Use Maclaurin series to approximate the following functions:

$$f(x) = \sin x$$

$$f(x) = \cos x$$

$$f(x) = \sin 2x + \cos 2x$$

Power Series

$$f(x)$$

$$\begin{aligned} &= a_0 + a_1(x - x_0)^1 \\ &+ a_2(x - x_0)^2 + a_3(x - x_0)^3 \\ &+ \cdots + a_n(x - x_0)^n + \cdots \end{aligned}$$

□ $f(x)$ and x_0 are given

□ where the constants a_0, a_1, a_2, \dots are called
coefficients of the power series

□ When $x_0 = 0$

$$f(x) = a_0 + a_1x + a_2x^2 + a_3x^3 + a_4x^4 + \dots$$

Example

□ Find a **power series** for the function

$$f(x) = e^x$$

$$f(x) = a_0 + a_1x + a_2x^2 + a_3x^3 + a_4x^4 + \dots$$

$$f(x) = a_0 + a_1x + a_2x^2 + a_3x^3 + a_4x^4 + \dots$$

$$\begin{array}{ll} f(x) = a_0 + a_1x + a_2x^2 + a_3x^3 + a_4x^4 + \dots & \rightarrow f(0) = a_0 \\ f'(x) = a_1 + 2a_2x + 3a_3x^2 + 4a_4x^3 + \dots & \rightarrow f'(0) = a_1 \\ f''(x) = 2a_2 + 6a_3x + 12a_4x^2 + \dots & \rightarrow f''(0) = 2a_2 \\ f'''(x) = 6a_3 + 24a_4x + \dots & \rightarrow f'''(0) = 6a_3 \end{array}$$

On the other hand

$$f(x) = e^x \quad \rightarrow \quad f(0) = e^0 = 1$$

$$f'(x) = e^x \quad \rightarrow \quad f'(0) = e^0 = 1$$

$$f''(x) = e^x \quad \rightarrow \quad f''(0) = e^0 = 1$$

$$a_0 = 1, \quad a_1 = 1, \quad a_2 = \frac{1}{2}, \quad a_3 = \frac{1}{6}$$

Thus, the function can be approximated as:

$$f(x) = a_0 + a_1x + a_2x^2 + a_3x^3 + a_4x^4 + \dots$$

$$f(x) = e^x = \sum_{n=0}^{\infty} \frac{x^n}{n!} = 1 + x + \frac{1}{2} x^2 + \frac{1}{6} x^3 + \dots$$

Example

□ Find a **power series** for the function

$$f(x) = \sqrt[3]{x+1}$$

$$f(x) = a_0 + a_1x + a_2x^2 + a_3x^3 + a_4x^4 + \dots$$

$$f(x) = a_0 + a_1x + a_2x^2 + a_3x^3 + a_4x^4 + \dots$$

$$\begin{array}{ll} f(x) = a_0 + a_1x + a_2x^2 + a_3x^3 + a_4x^4 + \dots & \rightarrow f(0) = a_0 \\ f'(x) = a_1 + 2a_2x + 3a_3x^2 + 4a_4x^3 + \dots & \rightarrow f'(0) = a_1 \\ f''(x) = 2a_2 + 6a_3x + 12a_4x^2 + \dots & \rightarrow f''(0) = 2a_2 \\ f'''(x) = 6a_3 + 24a_4x + \dots & \rightarrow f'''(0) = 6a_3 \end{array}$$

On the other hand

$$\begin{aligned} f(x) &= \sqrt[3]{x+1} & \rightarrow f(0) &= 1 \\ f'(x) &= \frac{1}{3}(1+x)^{-\frac{2}{3}} & \rightarrow f'(0) &= \frac{1}{3} \\ f''(x) &= -\frac{2}{9}(1+x)^{-\frac{5}{3}} & \rightarrow f''(0) &= -\frac{2}{9} \\ f'''(x) &= \frac{10}{27}(1+x)^{-\frac{8}{3}} & \rightarrow f'''(0) &= \frac{10}{27} \end{aligned}$$

$$a_0 = 1, \quad a_1 = \frac{1}{3}, \quad a_2 = \frac{-1}{9}, \quad a_3 = \frac{5}{81}$$

Thus, the function can be approximated as:

$$f(x) = a_0 + a_1x + a_2x^2 + a_3x^3 + a_4x^4 + \dots$$

$$f(x) = \sqrt[3]{x+1} = 1 + \frac{1}{3}x + \frac{-1}{9}x^2 + \frac{5}{81}x^3 + \dots$$